pulse/lib/steel/pulse/Pulse.Prover.Substs.fst
@@ -11,180 +11,407 @@ module L = FStar.List.Tot
 
 module Env = Pulse.Typing.Env
 
-let rec nt_subst_st_comp_commutes (s:st_comp) (ss:nt_substs)
-  : Lemma (ensures nt_subst_st_comp s ss ==
-           { s with res = nt_subst_term s.res ss;
-                    pre = nt_subst_term s.pre ss;
-                    post = nt_subst_term s.post ss; })
-          (decreases L.length ss) =
-  match ss with
+let rec no_repeats (l:list var) : Type0 =
+  match l with
+  | [] -> True
+  | x::tl -> (~ (L.memP x tl)) /\ no_repeats tl  
+
+type ss_dom = l:list var { no_repeats l }
+
+type ss_map = m:Map.t var term {
+  forall (x:var). (~ (Map.contains m x)) ==> Map.sel m x == tm_unknown
+}
+
+let remove_map (m:ss_map) (x:var) =
+  Map.restrict (Set.complement (Set.singleton x)) (Map.upd m x tm_unknown)
+
+let rec is_dom (l:ss_dom) (m:ss_map) : Type0 =
+  match l with
+  | [] -> Set.equal (Map.domain m) Set.empty
+  | x::tl ->
+    Map.contains m x /\ is_dom tl (remove_map m x)
+
+let rec is_dom_mem (l:ss_dom) (m:ss_map)
+  : Lemma
+      (requires is_dom l m)
+      (ensures forall (x:var).{:pattern L.memP x l \/ Map.contains m x}
+                              L.memP x l <==> Map.contains m x)
+      [SMTPat (is_dom l m)] =
+  match l with
   | [] -> ()
-  | (NT x e)::tl ->
-    nt_subst_st_comp_commutes (subst_st_comp s [ NT x e ]) tl
+  | y::tl -> is_dom_mem tl (remove_map m y)
 
+noeq
+type ss_t = {
+  l : ss_dom;
+  m : m:ss_map { is_dom l m }
+}
 
-let rec nt_subst_comp_commutes (c:comp) (ss:nt_substs)
-  : Lemma (ensures (let r = nt_subst_comp c ss in
-           (C_Tot? c ==> r == C_Tot (nt_subst_term (comp_res c) ss)) /\
-           (C_ST? c ==> r == C_ST (nt_subst_st_comp (st_comp_of_comp c) ss)) /\
-           (C_STAtomic? c ==> r == C_STAtomic (nt_subst_term (comp_inames c) ss)
-                                              (nt_subst_st_comp (st_comp_of_comp c) ss)) /\
-           (C_STGhost? c ==> r == C_STGhost (nt_subst_term (comp_inames c) ss)
-                                            (nt_subst_st_comp (st_comp_of_comp c) ss))))
-          (decreases L.length ss) =
+let as_map (ss:ss_t) = ss.m
+
+let empty = { l = []; m = Map.const_on Set.empty tm_unknown }
+
+let is_dom_push
+  (l:ss_dom)
+  (m:ss_map { is_dom l m })
+  (x:var { ~ (Map.contains m x ) })
+  (t:term)
+  : Lemma (is_dom (x::l) (Map.upd m x t)) =
+
+  assert (Map.equal (remove_map (Map.upd m x t) x) m)
+
+let push
+  (uvs:env)
+  (ss:ss_t { ss `solves` uvs })
+  (x:var { Set.mem x (Env.dom uvs) /\ ~ (contains ss x) })
+  (t:term { Set.disjoint (freevars t) (Env.dom uvs) }) : ss':ss_t { ss' `solves` uvs } =
   
-  match ss with
+  is_dom_push ss.l ss.m x t;
+  { l = x::ss.l;
+    m = Map.upd ss.m x t }
+
+let tail (ss:ss_t { Cons? ss.l }) : ss_t =
+   { l = L.tl ss.l; m = remove_map ss.m (L.hd ss.l) }
+
+let rec push_ss
+  (uvs:env)
+  (ss1:ss_t { ss1 `solves` uvs })
+  (ss2:ss_t { ss2 `solves` uvs /\ Set.disjoint (dom ss1) (dom ss2) })
+  : Tot (ss':ss_t { ss' `solves` uvs })
+        (decreases L.length ss2.l) =
+  match ss2.l with
+  | [] -> ss1
+  | x::tl ->
+    push_ss uvs (push uvs ss1 x (Map.sel ss2.m x)) (tail ss2)
+
+let push_as_map (uvs:env) (ss1 ss2:ss_t)
+  : Lemma (requires ss1 `solves` uvs /\ ss2 `solves` uvs /\ Set.disjoint (dom ss1) (dom ss2))
+          (ensures as_map (push_ss uvs ss1 ss2) ==
+                   Map.concat (as_map ss1) (as_map ss2))
+          [SMTPat (as_map (push_ss uvs ss1 ss2))] = admit ()
+
+let rec remove_l (l:ss_dom) (x:var { L.memP x l })
+  : Pure ss_dom
+         (requires True)
+         (ensures fun r -> forall (y:var). L.memP y r <==> (L.memP y l /\ y =!= x)) =
+  match l with
+  | [] -> assert False; []
+  | y::tl ->
+    if y = x then tl
+    else y::(remove_l tl x)
+
+let rec is_dom_remove
+  (l:ss_dom)
+  (m:ss_map { is_dom l m })
+  (x:var { Map.contains m x })
+  : Lemma (is_dom (remove_l l x) (remove_map m x))
+          [SMTPat (remove_l l x); SMTPat (remove_map m x)] =
+ 
+  match l with
   | [] -> ()
-  | (NT x e)::tl ->
-    nt_subst_comp_commutes (subst_comp c [ NT x e ]) tl
+  | y::tl ->
+    if x = y then ()
+    else let t_y = Map.sel m y in
+         let m1 = remove_map m y in
+         is_dom_remove tl m1 x;
+         assert (is_dom (remove_l tl x) (remove_map m1 x));
+         is_dom_push (remove_l tl x) (remove_map m1 x) y t_y;
+         assert (Map.equal (Map.upd (remove_map m1 x) y t_y)
+                           (remove_map m x))
 
-let rec nt_subst_term_compose (t:term) (ss1 ss2:nt_substs)
-: Lemma (ensures nt_subst_term (nt_subst_term t ss1) ss2 ==
-                 nt_subst_term t (compose_nt_substs ss1 ss2))
-        (decreases L.length ss1) =
+let rec ss_term (t:term) (ss:ss_t) : Tot term (decreases L.length ss.l) =
+  match ss.l with
+  | [] -> t
+  | y::tl ->
+    let t = subst_term t [ NT y (Map.sel ss.m y) ] in
+    ss_term t (tail ss)
 
-match ss1 with
-| [] -> ()
-| (NT x e)::tl -> nt_subst_term_compose (subst_term t [ NT x e ]) tl ss2
+let rec ss_st_term (t:st_term) (ss:ss_t) : Tot st_term (decreases L.length ss.l) =
+  match ss.l with
+  | [] -> t
+  | y::tl ->
+    let t = subst_st_term t [ NT y (Map.sel ss.m y) ] in
+    ss_st_term t (tail ss)
 
-let rec nt_subst_st_term_compose (t:st_term) (ss1 ss2:nt_substs)
-: Lemma (ensures nt_subst_st_term (nt_subst_st_term t ss1) ss2 ==
-                 nt_subst_st_term t (compose_nt_substs ss1 ss2))
-        (decreases L.length ss1) =
+let rec ss_st_comp (s:st_comp) (ss:ss_t)
+  : Tot st_comp (decreases L.length ss.l) =
+  match ss.l with
+  | [] -> s
+  | y::tl ->
+    let s = subst_st_comp s [ NT y (Map.sel ss.m y) ] in
+    ss_st_comp s (tail ss)
 
-match ss1 with
-| [] -> ()
-| (NT x e)::tl -> nt_subst_st_term_compose (subst_st_term t [ NT x e ]) tl ss2
+let rec ss_comp (c:comp) (ss:ss_t)
+  : Tot comp (decreases L.length ss.l) =
+  match ss.l with
+  | [] -> c
+  | y::tl ->
+    let c = subst_comp c [ NT y (Map.sel ss.m y) ] in
+    ss_comp c (tail ss)
 
-let rec nt_subst_comp_compose (c:comp) (ss1 ss2:nt_substs)
-: Lemma (ensures nt_subst_comp (nt_subst_comp c ss1) ss2 ==
-                 nt_subst_comp c (compose_nt_substs ss1 ss2))
-        (decreases L.length ss1) =
+let rec ss_binder (b:binder) (ss:ss_t)
+  : Tot binder (decreases L.length ss.l) =
+  match ss.l with
+  | [] -> b
+  | y::tl ->
+    let b = subst_binder b [ NT y (Map.sel ss.m y) ] in
+    ss_binder b (tail ss)
 
-match ss1 with
-| [] -> ()
-| (NT x e)::tl -> nt_subst_comp_compose (subst_comp c [ NT x e ]) tl ss2
+let rec ss_env (g:env) (ss:ss_t)
+  : Tot (g':env { fstar_env g' == fstar_env g /\
+                  Env.dom g' == Env.dom g })
+        (decreases L.length ss.l) =
+  admit ();
+  match ss.l with
+  | [] -> g
+  | y::tl -> ss_env (subst_env g [ NT y (Map.sel ss.m y) ]) (tail ss)
 
-let coerce_eq (#a #b:Type) (x:a) (_:squash (a === b)) : y:b{y == x} = x
+let rec ss_st_comp_commutes (s:st_comp) (ss:ss_t)
+  : Lemma (ensures
+             ss_st_comp s ss ==
+             { s with res = ss_term s.res ss;
+                      pre = ss_term s.pre ss;
+                      post = ss_term s.post ss; })  // no shifting required
+          (decreases L.length ss.l)
+          [SMTPat (ss_st_comp s ss)] =
+  match ss.l with
+  | [] -> ()
+  | y::tl -> ss_st_comp_commutes (subst_st_comp s [ NT y (Map.sel ss.m y) ]) (tail ss)
 
-let rec st_typing_nt_substs
-  (g:env) (uvs:env) (g':env { pairwise_disjoint g uvs g' })
-  (#t:st_term) (#c:comp_st) (t_typing:st_typing (push_env g (push_env uvs g')) t c)
-  (ss:nt_substs { well_typed_ss g uvs ss })
-: Tot (st_typing (push_env g (nt_subst_env g' ss)) (nt_subst_st_term t ss) (nt_subst_comp c ss))
-      (decreases L.length ss) =
+let rec ss_comp_commutes (c:comp) (ss:ss_t)
+  : Lemma (ensures
+             (let r = ss_comp c ss in
+              (C_Tot? c ==> r == C_Tot (ss_term (comp_res c) ss)) /\
+              (C_ST? c ==> r == C_ST (ss_st_comp (st_comp_of_comp c) ss)) /\
+              (C_STAtomic? c ==> r == C_STAtomic (ss_term (comp_inames c) ss)
+                                                 (ss_st_comp (st_comp_of_comp c) ss)) /\
+              (C_STGhost? c ==> r == C_STGhost (ss_term (comp_inames c) ss)
+                                               (ss_st_comp (st_comp_of_comp c) ss))))
+          (decreases L.length ss.l)
+          [SMTPat (ss_comp c ss)] =
+  match ss.l with
+  | [] -> ()
+  | y::tl -> ss_comp_commutes (subst_comp c [ NT y (Map.sel ss.m y) ]) (tail ss)
 
-match bindings uvs with
-| [] ->
-  assert (equal (push_env uvs g') g');
-  t_typing
+let is_permutation _ (nts:nt_substs) (ss:ss_t) : Type0 =
+  magic ()
 
-| _ ->
-  let x, ty, uvs' = remove_binding uvs in
-  let (NT y e)::ss' = ss in
-  let e_typing = FStar.IndefiniteDescription.elim_squash #(tot_typing g e ty) () in
-  push_env_assoc (singleton_env (fstar_env uvs) x ty) uvs' g';
-  let t_typing
-    : st_typing (push_env g (push_env (singleton_env (fstar_env g) x ty) (push_env uvs' g'))) t c
-    = coerce_eq t_typing () in
-  let t_typing
-    : st_typing (push_env g (subst_env (push_env uvs' g') [ NT y e ]))
-                (subst_st_term t [ NT y e ])
-                (subst_comp c [ NT y e ])
-    = st_typing_subst g x ty (push_env uvs' g') e_typing t_typing in
+let rec ss_to_nt_substs (g:env) (uvs:env) (ss:ss_t)
+  : T.Tac (option (nts:nt_substs { well_typed_nt_substs g uvs nts /\
+                                   is_permutation uvs nts ss })) =
+  
+  match bindings uvs with
+  | [] -> assume (is_permutation uvs [] ss); Some []
+  | _ ->
+    let x, ty, rest_uvs = remove_binding uvs in
+    if Map.contains ss.m x
+    then let t = Map.sel ss.m x in
+         let d : tot_typing g t ty = magic () in
+         let _ = FStar.Squash.return_squash d in
+         let nts_opt =
+           ss_to_nt_substs g (subst_env rest_uvs [ NT x t ]) {l=remove_l ss.l x;
+                                                              m=remove_map ss.m x} in
+         match nts_opt with
+         | None -> None
+         | Some nts ->
+           let nts : nts:nt_substs { well_typed_nt_substs g uvs nts } = (NT x t)::nts in
+           assume (is_permutation uvs nts ss);
+           Some nts
+    else None
 
-  assume (subst_env (push_env uvs' g') [ NT y e ] ==
-          push_env (subst_env uvs' [ NT y e ]) (subst_env g' [ NT y e ]));
+let ss_nt_subst (uvs:env) (ss:ss_t) (nts:nt_substs)
+  : Lemma (requires is_permutation uvs nts ss)
+          (ensures
+             (forall (t:term). nt_subst_term t nts == ss_term t ss) /\
+             (forall (b:binder). nt_subst_binder b nts == ss_binder b ss) /\
+             (forall (t:st_term). nt_subst_st_term t nts == ss_st_term t ss) /\
+             (forall (c:comp). nt_subst_comp c nts == ss_comp c ss) /\
+             (forall (s:st_comp). nt_subst_st_comp s nts == ss_st_comp s ss)) = admit ()
 
-  st_typing_nt_substs g
-    (subst_env uvs' [ NT y e ])
-    (subst_env g' [ NT y e ])
-    t_typing ss'
 
-let vprop_equiv_nt_substs
-  (g:env) (uvs:env) (g':env { pairwise_disjoint g uvs g' })
-  (#p1 #p2:vprop) (veq:vprop_equiv (push_env g (push_env uvs g')) p1 p2)
-  (ss:nt_substs { well_typed_ss g uvs ss })
-: vprop_equiv (push_env g (nt_subst_env g' ss)) (nt_subst_term p1 ss) (nt_subst_term p2 ss) =
+// let well_typed_nt_substs 
 
-admit ()
+// let permutation #uvs (ss1 ss2:ss_t uvs) =
+//   Map.equal ss1.m ss2.m
+
+// let rec ss_term_permutation #uvs (t:term) (ss1 ss2:ss_t uvs)
+//   : Lemma (requires permutation ss1 ss2)
+//           (ensures ) 
+
+// let rec nt_subst_st_comp_commutes (s:st_comp) (ss:nt_substs)
+//   : Lemma (ensures nt_subst_st_comp s ss ==
+//            { s with res = nt_subst_term s.res ss;
+//                     pre = nt_subst_term s.pre ss;
+//                     post = nt_subst_term s.post ss; })
+//           (decreases L.length ss) =
+//   match ss with
+//   | [] -> ()
+//   | (NT x e)::tl ->
+//     nt_subst_st_comp_commutes (subst_st_comp s [ NT x e ]) tl
+
+
+// let rec nt_subst_comp_commutes (c:comp) (ss:nt_substs)
+//   : Lemma (ensures (let r = nt_subst_comp c ss in
+//            (C_Tot? c ==> r == C_Tot (nt_subst_term (comp_res c) ss)) /\
+//            (C_ST? c ==> r == C_ST (nt_subst_st_comp (st_comp_of_comp c) ss)) /\
+//            (C_STAtomic? c ==> r == C_STAtomic (nt_subst_term (comp_inames c) ss)
+//                                               (nt_subst_st_comp (st_comp_of_comp c) ss)) /\
+//            (C_STGhost? c ==> r == C_STGhost (nt_subst_term (comp_inames c) ss)
+//                                             (nt_subst_st_comp (st_comp_of_comp c) ss))))
+//           (decreases L.length ss) =
+  
+//   match ss with
+//   | [] -> ()
+//   | (NT x e)::tl ->
+//     nt_subst_comp_commutes (subst_comp c [ NT x e ]) tl
+
+// let rec nt_subst_term_compose (t:term) (ss1 ss2:nt_substs)
+// : Lemma (ensures nt_subst_term (nt_subst_term t ss1) ss2 ==
+//                  nt_subst_term t (compose_nt_substs ss1 ss2))
+//         (decreases L.length ss1) =
+
+// match ss1 with
+// | [] -> ()
+// | (NT x e)::tl -> nt_subst_term_compose (subst_term t [ NT x e ]) tl ss2
+
+// let rec nt_subst_st_term_compose (t:st_term) (ss1 ss2:nt_substs)
+// : Lemma (ensures nt_subst_st_term (nt_subst_st_term t ss1) ss2 ==
+//                  nt_subst_st_term t (compose_nt_substs ss1 ss2))
+//         (decreases L.length ss1) =
+
+// match ss1 with
+// | [] -> ()
+// | (NT x e)::tl -> nt_subst_st_term_compose (subst_st_term t [ NT x e ]) tl ss2
+
+// let rec nt_subst_comp_compose (c:comp) (ss1 ss2:nt_substs)
+// : Lemma (ensures nt_subst_comp (nt_subst_comp c ss1) ss2 ==
+//                  nt_subst_comp c (compose_nt_substs ss1 ss2))
+//         (decreases L.length ss1) =
+
+// match ss1 with
+// | [] -> ()
+// | (NT x e)::tl -> nt_subst_comp_compose (subst_comp c [ NT x e ]) tl ss2
+
+// let coerce_eq (#a #b:Type) (x:a) (_:squash (a === b)) : y:b{y == x} = x
+
+// let rec st_typing_nt_substs
+//   (g:env) (uvs:env) (g':env { pairwise_disjoint g uvs g' })
+//   (#t:st_term) (#c:comp_st) (t_typing:st_typing (push_env g (push_env uvs g')) t c)
+//   (ss:nt_substs { well_typed_ss g uvs ss })
+// : Tot (st_typing (push_env g (nt_subst_env g' ss)) (nt_subst_st_term t ss) (nt_subst_comp c ss))
+//       (decreases L.length ss) =
+
+// match bindings uvs with
+// | [] ->
+//   assert (equal (push_env uvs g') g');
+//   t_typing
+
+// | _ ->
+//   let x, ty, uvs' = remove_binding uvs in
+//   let (NT y e)::ss' = ss in
+//   let e_typing = FStar.IndefiniteDescription.elim_squash #(tot_typing g e ty) () in
+//   push_env_assoc (singleton_env (fstar_env uvs) x ty) uvs' g';
+//   let t_typing
+//     : st_typing (push_env g (push_env (singleton_env (fstar_env g) x ty) (push_env uvs' g'))) t c
+//     = coerce_eq t_typing () in
+//   let t_typing
+//     : st_typing (push_env g (subst_env (push_env uvs' g') [ NT y e ]))
+//                 (subst_st_term t [ NT y e ])
+//                 (subst_comp c [ NT y e ])
+//     = st_typing_subst g x ty (push_env uvs' g') e_typing t_typing in
+
+//   assume (subst_env (push_env uvs' g') [ NT y e ] ==
+//           push_env (subst_env uvs' [ NT y e ]) (subst_env g' [ NT y e ]));
+
+//   st_typing_nt_substs g
+//     (subst_env uvs' [ NT y e ])
+//     (subst_env g' [ NT y e ])
+//     t_typing ss'
+
+// let vprop_equiv_nt_substs
+//   (g:env) (uvs:env) (g':env { pairwise_disjoint g uvs g' })
+//   (#p1 #p2:vprop) (veq:vprop_equiv (push_env g (push_env uvs g')) p1 p2)
+//   (ss:nt_substs { well_typed_ss g uvs ss })
+// : vprop_equiv (push_env g (nt_subst_env g' ss)) (nt_subst_term p1 ss) (nt_subst_term p2 ss) =
+
+// admit ()
 
 let vprop_equiv_nt_substs_derived _ _ _ _ = admit ()
 
 
-type map = m:Map.t var term {
-  forall (x:var). (~ (Map.contains m x)) ==> Map.sel m x == tm_unknown
-}
+// type map = m:Map.t var term {
+//   forall (x:var). (~ (Map.contains m x)) ==> Map.sel m x == tm_unknown
+// }
 
-let related (l:list (var & term)) (m:map) =
-  (forall (b:var & term).
-          L.memP b l ==> (Map.contains m (fst b) /\
-                          Map.sel m (fst b) == snd b)) /\
+// let related (l:list (var & term)) (m:map) =
+//   (forall (b:var & term).
+//           L.memP b l ==> (Map.contains m (fst b) /\
+//                           Map.sel m (fst b) == snd b)) /\
   
-  (forall (x:var). Map.contains m x ==> L.memP (x, Map.sel m x) l)
+//   (forall (x:var). Map.contains m x ==> L.memP (x, Map.sel m x) l)
 
-noeq
-type t = {
-  l : list (var & term);
-  m : m:map { related l m }
-}
+// noeq
+// type t = {
+//   l : list (var & term);
+//   m : m:map { related l m }
+// }
 
-let rec as_nt_substs_aux (l:list (var & term)) : nt_substs =
-  match l with
-  | [] -> []
-  | (x, t)::tl -> (NT x t)::(as_nt_substs_aux tl)
+// let rec as_nt_substs_aux (l:list (var & term)) : nt_substs =
+//   match l with
+//   | [] -> []
+//   | (x, t)::tl -> (NT x t)::(as_nt_substs_aux tl)
 
-let as_nt_substs s = as_nt_substs_aux s.l
+// let as_nt_substs s = as_nt_substs_aux s.l
 
-let as_map s = s.m
+// let as_map s = s.m
 
-let empty = {
-  l = [];
-  m = Map.const_on Set.empty tm_unknown;
-}
+// let empty = {
+//   l = [];
+//   m = Map.const_on Set.empty tm_unknown;
+// }
 
-let empty_dom () = assert (Set.equal (dom empty) Set.empty)
+// let empty_dom () = assert (Set.equal (dom empty) Set.empty)
 
-let singleton (x:var) (t:term) = {
-  l = [ (x, t) ];
-  m = Map.upd (Map.const_on Set.empty tm_unknown) x t;
-}
+// let singleton (x:var) (t:term) = {
+//   l = [ (x, t) ];
+//   m = Map.upd (Map.const_on Set.empty tm_unknown) x t;
+// }
 
-//
-// TODO: Move to ulib
-//
-let rec append_memP (#a:Type) (l1 l2:list a) (x:a)
-  : Lemma (L.memP x (l1 @ l2) <==> (L.memP x l1 \/ L.memP x l2))
-          [SMTPat (L.memP x (l1 @ l2))] =
-  match l1 with
-  | [] -> ()
-  | _::tl -> append_memP tl l2 x
+// //
+// // TODO: Move to ulib
+// //
+// let rec append_memP (#a:Type) (l1 l2:list a) (x:a)
+//   : Lemma (L.memP x (l1 @ l2) <==> (L.memP x l1 \/ L.memP x l2))
+//           [SMTPat (L.memP x (l1 @ l2))] =
+//   match l1 with
+//   | [] -> ()
+//   | _::tl -> append_memP tl l2 x
 
-let push s1 s2 = {
-  l = s1.l @ s2.l;
-  m = Map.concat s1.m s2.m;
-}
+// let push s1 s2 = {
+//   l = s1.l @ s2.l;
+//   m = Map.concat s1.m s2.m;
+// }
 
-let push_as_map _ _ = ()
+// let push_as_map _ _ = ()
 
-let check_well_typedness g uvs ss = admit (); true
+// let check_well_typedness g uvs ss = admit (); true
 
-// let t _ = magic ()
-// let as_subst _ = magic ()
-// let as_map _ = magic ()
-// let subst_as_map _ = admit ()
-// let equal_elim _ _ = admit ()
-// let empty _ = magic ()
-// let empty_dom _ = admit ()
-// let singleton _ = magic ()
-// let singleton_dom _ _ = admit ()
-// let push _ _ = magic ()
-// let push_substs_as_map _ _ = admit ()
-// let push_subst_term _ _ _ = admit ()
-// let push_subst_st_term _ _ _ = admit ()
-// let push_subst_comp _ _ _ = admit ()
-// let subst_closed_term _ _ = admit ()
-// let subst_closed_st_term _ _ = admit ()
-// let subst_closed_comp _ _ = admit ()
-// let diff _ _ = magic ()
-// let diff_push _ _ = admit ()
+// // let t _ = magic ()
+// // let as_subst _ = magic ()
+// // let as_map _ = magic ()
+// // let subst_as_map _ = admit ()
+// // let equal_elim _ _ = admit ()
+// // let empty _ = magic ()
+// // let empty_dom _ = admit ()
+// // let singleton _ = magic ()
+// // let singleton_dom _ _ = admit ()
+// // let push _ _ = magic ()
+// // let push_substs_as_map _ _ = admit ()
+// // let push_subst_term _ _ _ = admit ()
+// // let push_subst_st_term _ _ _ = admit ()
+// // let push_subst_comp _ _ _ = admit ()
+// // let subst_closed_term _ _ = admit ()
+// // let subst_closed_st_term _ _ = admit ()
+// // let subst_closed_comp _ _ = admit ()
+// // let diff _ _ = magic ()
+// // let diff_push _ _ = admit ()
